removed matchable and Is_MM ->  MM_in

Matching.v
@@ -21,20 +21,15 @@ Section Matching.
   
 (*----------------- Notion of matching and  Maximal Matching (MM) ------------------------*)
 
-Definition matchable (b: Bid)(a: Ask):=  (sp (a)) <= (bp (b)).
+(* Definition matchable (b: Bid)(a: Ask):=  (sp (a)) <= (bp (b)). *)
 
-Check matchable.
-
-Definition All_matchable (M: list fill_type):= forall m, In m M -> matchable (bid_of m) (ask_of m).
+Definition All_matchable (M: list fill_type):= forall m, In m M -> (ask_of m) <= (bid_of m).
 
 Definition all_matchable (M:list fill_type) := forallb (fun m => 
  (bid_of m) <=? (ask_of m)) M.
 
 Lemma all_matchableP (M:list fill_type): reflect (All_matchable M) (all_matchable M).
-Proof. unfold All_matchable. unfold all_matchable.  
-Admitted.
-
-Hint Unfold All_matchable.
+Proof.  Admitted.
 
 Definition matching (M: list fill_type):=
   (All_matchable M) /\ (NoDup (bids_of M)) /\ (NoDup (asks_of M)).
@@ -42,14 +37,14 @@ Definition matching (M: list fill_type):=
 Definition matching_in (B:list Bid) (A:list Ask) (M:list fill_type):=
 (matching M) /\ ((bids_of M) [<=] B) /\ ((asks_of M) [<=] A).
 
-Definition Is_MM (M : list fill_type) (B: list Bid) (A: list Ask):=
+Definition MM_in (B: list Bid)(A: list Ask)(M : list fill_type) :=
   matching_in B A M /\ 
   (forall M': list fill_type, matching_in B A M'-> |M'| <= |M|).
 
 
 Lemma All_matchable_elim (m: fill_type)(M: list fill_type):
-  All_matchable (m::M) -> matchable (bid_of m) (ask_of m).
-Proof.  intros H.  unfold All_matchable in H. simpl in H. specialize H with m. auto. Qed.   
+  All_matchable (m::M) -> (ask_of m) <= (bid_of m).
+Proof.  intros H.  unfold All_matchable in H. simpl in H. auto.  Qed.   
  
 
 Lemma All_matchable_elim1 (m: fill_type)(M: list fill_type):
@@ -59,20 +54,22 @@ Proof.  unfold All_matchable. intros.  simpl in H. auto. Qed.
 Definition empty_fill: list fill_type:= nil.
 
 Lemma All_matchable_nil: All_matchable nil.
-Proof. unfold All_matchable.
-intros. inversion H. Qed.  
+Proof. unfold All_matchable. intros. inversion H. Qed.  
 
 Lemma All_matchable_intro (m: fill_type)(M: list fill_type):
-  matchable (bid_of m) (ask_of m) -> All_matchable M -> All_matchable (m::M).
-Proof. intros H1 H2. unfold All_matchable. simpl. intros m0 H3. destruct H3. subst m0. exact. eauto. Qed. 
+  (ask_of m) <= (bid_of m) -> All_matchable M -> All_matchable (m::M).
+Proof. { intros H1 H2. unfold All_matchable. simpl. intros m0 H3. destruct H3.
+         subst m0. exact. eauto. } Qed. 
 
 
 Hint Immediate All_matchable_intro All_matchable_nil: auction.
 Hint Resolve All_matchable_elim All_matchable_elim1 : auction.
 
 Lemma nill_is_matching (B: list Bid)(A: list Ask) : matching_in B A nil.
-Proof.  unfold matching_in. split. unfold matching. split. apply All_matchable_nil. split. 
-simpl. constructor. simpl. constructor. split. simpl. auto. simpl. auto. Qed.
+Proof. { unfold matching_in. split. unfold matching.
+         split. apply All_matchable_nil.
+         split. simpl. constructor. simpl. constructor.
+         split. simpl. auto. simpl. auto. } Qed.
 
 
 Hint Resolve nill_is_matching: auction.
@@ -80,9 +77,10 @@ Hint Resolve nill_is_matching: auction.
 
 
 Lemma matching_in_intro (m: fill_type) (M: list fill_type)(B: list Bid)(A: list Ask):
-  matchable (bid_of m)(ask_of m) -> matching_in B A M -> ~ In (bid_of m) (bids_of M) ->
+  (ask_of m) <= (bid_of m) -> matching_in B A M -> ~ In (bid_of m) (bids_of M) ->
   ~ In (ask_of m) (asks_of M) -> In (bid_of m) B -> In (ask_of m) A -> matching_in B A (m::M).
   Proof. Admitted.
+
   (*
 Proof.  intros H1 H2 H3 H4 H5 H6. unfold Is_a_matching. split. unfold Is_a_matching in H2. destruct H2. eauto with auction. split. unfold Is_a_matching in H2. destruct H2 as [H7 H2]. destruct H2 as [H8 H2]. destruct H2 as [H9 H2]. destruct H2 as [H10 H2]. simpl. eauto. split. destruct H2 as [H7 H2]. destruct H2 as [H8 H2]. destruct H2 as [H9 H2]. destruct H2 as [H10 H2]. simpl. eauto. split. destruct H2 as [H7 H2]. destruct H2 as [H8 H2]. destruct H2 as [H9 H2]. destruct H2 as [H10 H2]. simpl. unfold "[<=]". simpl. intros a H. destruct H.  subst a. exact. eauto. destruct H2 as [H7 H2]. destruct H2 as [H8 H2]. destruct H2 as [H9 H2]. destruct H2 as [H10 H2]. simpl. unfold "[<=]". simpl. intros a H. destruct H.  subst a. exact. eauto. Qed.
 
@@ -96,56 +94,57 @@ Proof. unfold Is_a_matching. simpl. intros H. destruct H as [H1 H]. destruct H a
 *)
 
 Lemma matching_in_elim1 (m: fill_type) (M: list fill_type) (B: list Bid)(A: list Ask):
-  matching_in B A (m::M) ->  matchable (bid_of m )(ask_of m).
-Proof. unfold matching_in. unfold matching. intros H. destruct H as [H1 H]. destruct H1 as [H1 H2]. eauto. Qed.
+  matching_in B A (m::M) ->  (ask_of m) <= (bid_of m).
+Proof. unfold matching_in. intros H. destruct H as [H1 H]. destruct H1 as [H1 H2]. eauto. Qed.
  
 
 Lemma matching_in_elim2 (m: fill_type) (M: list fill_type) (B: list Bid)(A: list Ask):
   matching_in B A (m::M) ->   ~ In (bid_of m) (bids_of M).
-Proof.  unfold matching_in;unfold matching. intros H. destruct H as [H1 H]. destruct H as [H2 H]. destruct H1 as [H1 H3]. destruct H3 as [H3 H4]. simpl in H2. eauto. Qed.
+Proof. { unfold matching_in;unfold matching. intros H.
+         destruct H as [H1 H]. destruct H as [H2 H]. destruct H1 as [H1 H3].
+         destruct H3 as [H3 H4]. eauto. } Qed.
 
 
 Lemma matching_in_elim3 (m: fill_type) (M: list fill_type) (B: list Bid)(A: list Ask):
   matching_in B A (m::M) ->   ~ In (ask_of m) (asks_of M).
-Proof. unfold matching_in;unfold matching. intros H. destruct H as [H1 H]. destruct H as [H2 H]. destruct H1 as [H1 H3]. destruct H3 as [H3 H4]. simpl in H3. eauto. Qed.
+Proof. { unfold matching_in;unfold matching. intros H.
+         destruct H as [H1 H]. destruct H as [H2 H]. destruct H1 as [H1 H3].
+         destruct H3 as [H3 H4]. eauto. } Qed.
 
 Lemma matching_in_elim4 (m: fill_type) (M: list fill_type) (B: list Bid)(A: list Ask):
   matching_in B A (m::M) ->   In (bid_of m) B.
-Proof. unfold matching_in;unfold matching. intros H. destruct H as [H1 H]. destruct H as [H2 H]. destruct H1 as [H1 H3]. destruct H3 as [H3 H4]. simpl in H4. eauto. Qed.
+Proof. { unfold matching_in;unfold matching. intros H.
+         destruct H as [H1 H]. destruct H as [H2 H]. destruct H1 as [H1 H3].
+         destruct H3 as [H3 H4]. eauto. } Qed.
 
 Lemma matching_in_elim5 (m: fill_type) (M: list fill_type) (B: list Bid)(A: list Ask):
   matching_in B A (m::M) ->   In (ask_of m) A.
-Proof. unfold matching_in;unfold matching. intros H. destruct H as [H1 H]. destruct H as [H2 H]. destruct H1 as [H1 H3]. destruct H3 as [H3 H4]. simpl in H. eauto. Qed.
-
-(* Remove_later
-
-Variable m_by_bp m_by_sp : fill_type->fill_type-> bool.
-Variable b_by_bp : Bid -> Bid->bool.
-Variable a_by_sp : Ask -> Ask->bool.
-
-
-
-
-Lemma sorted_mbp_is_matching (M:list fill_type)(B:list Bid)(A:list Ask):
-matching_in B A M -> matching_in (sort m_by_bp M) B A.
-Proof. Admitted.
-
-Lemma sorted_msp_is_matching (M:list fill_type)(B:list Bid)(A:list Ask):
-matching_in B A M -> matching_in (sort m_by_sp M) B A.
-Proof. Admitted.
-
-Lemma sorted_bid_is_matching (M:list fill_type)(B:list Bid)(A:list Ask):
-matching_in B A M -> matching_in M (sort b_by_bp B) A.
-Proof. Admitted.
-
-Lemma sorted_ask_is_matching (M:list fill_type)(B:list Bid)(A:list Ask):
-matching_in B A M -> matching_in M B (sort a_by_sp A).
-Proof. Admitted. *)
+Proof. { unfold matching_in;unfold matching. intros H.
+         destruct H as [H1 H]. destruct H as [H2 H]. destruct H1 as [H1 H3].
+         destruct H3 as [H3 H4]. eauto. } Qed.
 
 Hint Immediate matching_in_intro: auction.
 Hint Resolve matching_in_elim matching_in_elim1 matching_in_elim2
      matching_in_elim3 matching_in_elim4 matching_in_elim5: auction.
- (* Remove_later    
+
+(* Remove_later
+Variable m_by_bp m_by_sp : fill_type->fill_type-> bool.
+Variable b_by_bp : Bid -> Bid->bool.
+Variable a_by_sp : Ask -> Ask->bool.
+
+Lemma sorted_mbp_is_matching (M:list fill_type)(B:list Bid)(A:list Ask):
+matching_in B A M -> matching_in (sort m_by_bp M) B A.
+Proof. Admitted.
+Lemma sorted_msp_is_matching (M:list fill_type)(B:list Bid)(A:list Ask):
+matching_in B A M -> matching_in (sort m_by_sp M) B A.
+Proof. Admitted.
+Lemma sorted_bid_is_matching (M:list fill_type)(B:list Bid)(A:list Ask):
+matching_in B A M -> matching_in M (sort b_by_bp B) A.
+Proof. Admitted.
+Lemma sorted_ask_is_matching (M:list fill_type)(B:list Bid)(A:list Ask):
+matching_in B A M -> matching_in M B (sort a_by_sp A).
+Proof. Admitted. *)
+(* Remove_later    
 Hint Resolve sorted_mbp_is_matching sorted_msp_is_matching sorted_bid_is_matching sorted_ask_is_matching : auction.
 *)
 
@@ -156,7 +155,8 @@ Definition rational (m: fill_type):=
 Definition Is_IR (M: list fill_type):= forall m, In m M -> rational m.
 
 Lemma Is_IR_elim (m: fill_type)(M: list fill_type): Is_IR (m::M) -> rational m.
-Proof. unfold Is_IR. intros H.  specialize H with m. simpl in H. destruct H. left. exact. unfold rational. eauto. Qed.
+Proof. { unfold Is_IR. intros H.  specialize H with m. simpl in H.
+         destruct H. left. exact. unfold rational. eauto. } Qed.
 
 Lemma Is_IR_elim1 (m: fill_type)(M: list fill_type): Is_IR (m::M)-> Is_IR M.
 Proof. unfold Is_IR. simpl. intros. eauto. Qed.
@@ -170,32 +170,22 @@ Hint Resolve Is_IR_elim Is_IR_elim1: auction.
 Definition fair_on_bids (M: list fill_type)(B: list Bid):=
   (forall b b', In b B /\ In b' B -> b > b' -> In b' (bids_of M) -> In b (bids_of M)).
 
-
 Definition fair_on_asks (M: list fill_type) (A: list Ask):=
   (forall s s', In s A /\ In s' A -> s < s' -> In s' (asks_of M) -> In s (asks_of M)).
 
-  
 Definition Is_fair (M: list fill_type) (B: list Bid) (A: list Ask) 
   :=  fair_on_asks M A /\ fair_on_bids M B.
 
-
 (* Remove_later
-
 Lemma sorted_mbp_is_fair (M:list fill_type)(B:list Bid)(A:list Ask):
 Is_fair M B A -> Is_fair (sort m_by_bp M) B A.
 Proof. Admitted.
-
-
 Lemma sorted_msp_is_fair (M:list fill_type)(B:list Bid)(A:list Ask):
 Is_fair M B A -> Is_fair (sort m_by_sp M) B A.
 Proof. Admitted.
-
-
 Lemma sorted_bid_is_fair (M:list fill_type)(B:list Bid)(A:list Ask):
 Is_fair M B A -> Is_fair M (sort b_by_bp B) A.
 Proof. Admitted.
-
-
 Lemma sorted_ask_is_fair (M:list fill_type)(B:list Bid)(A:list Ask):
 Is_fair M B A -> Is_fair M B (sort a_by_sp A).
 Proof. Admitted.
